relations.v
@@ -3,6 +3,7 @@ From RelationAlgebra Require Import lattice monoid rel kat_tac.
 From mathcomp Require Import ssreflect ssrbool ssrfun eqtype seq order choice.
 From mathcomp Require Import finmap fingraph fintype finfun ssrnat path.
 From Equations Require Import Equations.
+From monae Require Import hierarchy monad_model.
 From event_struct Require Import utilities wftype monad.
 
 (******************************************************************************)
@@ -38,29 +39,74 @@ Set Equations Transparent.
 Import Order.LTheory.
 Local Open Scope order_scope.
 Local Open Scope ra_terms.
+Local Open Scope monae_scope.
 
-Definition sfrel {T : eqType} (f : T -> seq T) : rel T :=
-  [rel a b | a \in f b].
-
+Definition sfrel {M : nondetMonad} {η : M ≈> ModelNondet.list}
+  {T : eqType} (f : T -> M T) : rel T :=
+    [rel a b | a \in η T (f b)].
 
 
 Section Strictify.
 
-Context {T : eqType}.
-Implicit Type (f : T -> seq T).
+Context (T : eqType).
+Variable  (M : nondetMonad) (η : M ≈> ModelNondet.list).
+Implicit Type (f : T -> M T).
 
-Definition strictify f : T -> seq T :=
-  fun x => filter^~ (f x) (fun y => y != x).
+Definition mfilter (s : M T) (p : pred T) :=
+  s >>= (fun a => if p a then Ret a else Fail).
+
+Lemma mem_ret (x : T) :
+  η T (Ret x) = [:: x].
+Proof.
+  have: η T (Ret x) = (η T \o Ret) x.
+  { done. }
+  move=> ->. by rewrite ret_morph /Ret /= /ModelMonad.ListMonad.ret_component.
+Qed.
+
+Lemma mem_fail :
+  η T Fail = [::].
+Proof. by rewrite fail_morph. Qed.
+
+Lemma mem_ret_eq (x y : T) :
+  x \in η T (Ret y) = (x == y).
+Proof.
+  have: η T (Ret y) = (η T \o Ret) y.
+  { done. }
+  move=> ->. rewrite ret_morph in_cons in_nil. by case: (x == y).
+Qed.
+
+Lemma mem_mfilter (p : pred T) (x : T) (s : M T) :
+  (x \in η T (mfilter s p)) = p x && (x \in η T s).
+Proof.
+  rewrite /mfilter bind_morph /Bind.
+  rewrite /ModelNondet.list /= /Actm /=.
+  rewrite /monad_lib.Monad_of_ret_bind.Map /ModelMonad.ListMonad.bind.
+  rewrite /ModelMonad.ListMonad.ret /ModelMonad.ListMonad.ret_component /=.
+  rewrite /comp. apply /flatten_mapP.
+  case: ifP => /andP.
+  { move=> [px xs]. exists [:: x]; last exact: mem_head.
+    apply /flatten_mapP. exists x => //=.
+    by rewrite px mem_ret mem_head. }
+  move=> H [] l /flatten_mapP [] y ys lh xl.
+  move: H => []. case H: (p y).
+  { move: lh. rewrite H mem_ret mem_seq1 => /eqP ly.
+    move: xl. by rewrite ly mem_seq1 => /eqP ->. }
+  move: lh. rewrite H mem_fail mem_seq1 => /eqP el.
+  by rewrite el in xl.
+Qed.
+
+Definition strictify f : T -> M T :=
+  fun x => mfilter (f x) (fun y => y != x).
 
 Lemma strictify_weq f :
-  sfrel (strictify f) ≡ (sfrel f \ eq_op).
+  @sfrel M η T (strictify f) ≡ (@sfrel M η T f \ eq_op).
 Proof. 
-  move=> x y; rewrite /sfrel /strictify /=.
-  by rewrite mem_filter andbC.
+  move=> x y; rewrite /sfrel /strictify /mfilter /=.
+  by rewrite mem_mfilter andbC.
 Qed.
 
 Lemma strictify_leq f : 
-  sfrel (strictify f) ≦ sfrel f.
+  @sfrel M η T (strictify f) ≦ @sfrel M η T f.
 Proof. by rewrite strictify_weq; lattice. Qed.
 
 End Strictify. 
@@ -71,10 +117,10 @@ Section WfRTClosure.
 
 Context {disp : unit} {T : wfType disp}.
 
-Variable (f : T -> seq T).
+Variable (M : nondetMonad) (η : M ≈> ModelNondet.list) (f : T -> M T).
 
 (* Hypothesis descend : forall x y, y \in f x -> y < x. *)
-Hypothesis descend : sfrel f ≦ (<%O).
+Hypothesis descend : @sfrel M η T f ≦ (<%O).
 
 (* A hack to get around a bug in Equations 
  * (see https://github.com/mattam82/Coq-Equations/issues/241).
@@ -82,56 +128,77 @@ Hypothesis descend : sfrel f ≦ (<%O).
  * (we can do it by adding `noind` specifier, but then we cannot use `funelim`).
  * Thus we have to "tie a recursive knot" manually. 
  *)
-Definition suffix_aux (x : T) (rec : forall y : T, y < x -> seq T) := 
+ Definition suffix_aux (x : T) (rec : forall y : T, y < x -> M T) := 
   let ys := f x in 
-  let ps := flatten (map^~ (seq_in ys) (fun y => 
-    rec (val y) (descend _ _ (valP y))
-  )) 
-  in ys ++ ps.
+  let ps := ys >>= (fun x => 
+  if x \in η T ys =P true is ReflectT pf then
+    rec x (descend _ _ pf)
+  else
+    Fail
+  ) in Alt ys ps.
 
 (* strict suffix of an element `x`, i.e. a set { y | x R y } *)
-Equations suffix (x : T) : seq T by wf x (<%O : rel T) := 
+Equations suffix (x : T) : M T by wf x (<%O : rel T) := 
   suffix x := suffix_aux x suffix.
 
 (* weak suffix of an element `x`, i.e. a set { y | x R? y } *)
-Definition wsuffix (x : T) : seq T :=
-  x :: suffix x.
+Definition wsuffix (x : T) : M T :=
+  Alt (Ret x) (suffix x).
 
 (* decidable transitive closure *)
 Definition t_closure : rel T := 
-  fun x y => x \in suffix y.
+  fun x y => x \in η T (suffix y).
 
 (* decidable reflexive-transitive closure *)
 Definition rt_closure : rel T := 
-  fun x y => x \in wsuffix y. 
-
+  fun x y => x \in η T (wsuffix y).
+  
 (* ************************************************************************** *)
 (*       THEORY                                                               *)
 (* ************************************************************************** *)
 
+Lemma mem_alt (x : T) (s1 s2 : M T) :
+  x \in η T (Alt s1 s2) = (x \in η T s1) || (x \in η T s2).
+Proof. by rewrite alt_morph mem_cat. Qed.
+
+Lemma bind_mapP (s : M T) (m : T -> M T) y :
+  reflect (exists2 x, x \in η T s & y \in η T (m x)) (y \in η T (s >>= m)).
+Proof.
+  apply /(iffP idP).
+  { rewrite bind_morph => /flatten_mapP.
+    move => [] l /flatten_mapP [] x xs.
+    rewrite mem_seq1 => /eqP -> ymx.
+    by exists x. }
+  move => [] x xs ymx. rewrite bind_morph.
+  apply /flatten_mapP. exists (η T (m x)) => //.
+  apply /flatten_mapP. exists x => //. exact: mem_head.
+Qed.
+
+Lemma strict_lt n k : k \in η T ((strictify T M f) n) -> k < n.
+Proof. by rewrite mem_mfilter lt_neqAle=> /andP[] -> /descend /ltW ->. Qed.
+
 Lemma t_closure_n1P x y : 
-  reflect (clos_trans_n1 T (sfrel f) x y) (t_closure x y).
+  reflect (clos_trans_n1 T (@sfrel M η T f) x y) (t_closure x y).
 Proof.
   rewrite /t_closure. funelim (suffix y)=> /=. 
-  apply /(iffP idP); rewrite mem_cat /sfrel /=.
-  { move=> /orP[|/flatten_mapP[z]] //; first exact: tn1_step.
-    move=> S /X H; apply: tn1_trans (valP z) _.
-    by apply: H=> //=; apply: descend (valP z). }
-  move: X=> /[swap] [[?->//|y ? /[dup] ? L /[swap]]].
-  move=> /[apply] H; apply/orP; right; apply/flatten_mapP.
-  eexists; first by apply: seq_in_mem L.
-  by apply /H=> //=; apply: descend.
+  apply /(iffP idP); rewrite mem_alt /sfrel /=.
+  { move=> /orP[|/bind_mapP[y]]; first exact: tn1_step.
+    case: eqP=> // S /descend yx /X tr. move: (tr y yx erefl) => H.
+    apply: tn1_trans; first by exact: S. done. }
+  move: X=> /[swap] [[?-> //|y z L /[swap]]].
+  move=> /[apply] H; apply/orP; right; apply/bind_mapP.
+  exists y=> //. case: eqP => // /descend yz. exact: H.
 Qed.
 
 Lemma t_closureP x y :
-  reflect (clos_trans T (sfrel f) x y) (t_closure x y).
+  reflect (clos_trans T (@sfrel M η T f) x y) (t_closure x y).
 Proof.
   apply /(equivP (t_closure_n1P x y)).
   symmetry; exact: clos_trans_tn1_iff.
 Qed.
 
 Lemma clos_trans_lt : 
-  clos_trans T (sfrel f) ≦ (<%O : rel T).
+  clos_trans T (@sfrel M η T f) ≦ (<%O : rel T).
 Proof. 
   move=> ??; rewrite/sfrel /=.
   elim=> [y z /descend | x y z _ ] //=.
@@ -153,21 +220,24 @@ Proof.
   apply /t_closureP /t_trans; eauto. 
 Qed.
 
+Ltac list_altP := rewrite /Alt /= /monae_lib.curry /= mem_cat.
+
 Lemma rt_closureP x y :
-  reflect (clos_refl_trans T (sfrel f) x y) (rt_closure x y).
+  reflect (clos_refl_trans T (@sfrel M η T f) x y) (rt_closure x y).
 Proof.
   apply /equivP; last first.
   { rewrite clos_refl_transE clos_reflE. 
     apply or_iff_compat_l; symmetry.
     apply rwP; exact: t_closureP. }
-  rewrite /t_closure /rt_closure /wsuffix in_cons.
+  rewrite /t_closure /rt_closure /wsuffix alt_morph. list_altP.
+  rewrite mem_ret_eq.
   by apply predU1P.
 Qed.
 
 Lemma rt_closureE : rt_closure ≡ eq_op ⊔ t_closure.
 Proof. 
   move=> x y /=; rewrite /rt_closure /t_closure. 
-  by rewrite /wsuffix in_cons eq_sym.
+  rewrite /wsuffix alt_morph. list_altP. by rewrite mem_ret_eq.
 Qed.
 
 Lemma rt_closure_le : rt_closure ≦ (<=%O : rel T).
@@ -178,7 +248,8 @@ Proof.
 Qed.
 
 Lemma rt_closure_refl x : rt_closure x x.
-Proof. exact: mem_head. Qed.
+Proof.
+  rewrite /rt_closure alt_morph. list_altP. by rewrite mem_ret_eq eq_refl. Qed.
 
 Lemma rt_closure_antisym : antisymmetric rt_closure.
 Proof.
@@ -247,11 +318,43 @@ Proof.
   by apply/equivsP; rewrite -map_comp -{1}(val_seq_in (f _)) -eq_in_map.
 Qed.
 
+Definition id_nattrans : ModelNondet.list ~> ModelNondet.list :=
+  Natural.Pack (Natural.Mixin (@monad_lib.natural_id _)).
+
+Lemma ret_id a : id_nattrans a \o Ret = Ret.
+Proof. by []. Qed.
+
+Lemma join_id a m : id_nattrans a (Join m) =
+  Join (id_nattrans (ModelNondet.list a) ((ModelNondet.list # id_nattrans a) m)).
+Proof.
+  rewrite /id_nattrans /= /ModelMonad.ListMonad.bind /ModelNondet.list /=.
+  rewrite /Actm /= /monad_lib.Monad_of_ret_bind.Map /=.
+  rewrite /ModelMonad.ListMonad.ret_component /ModelMonad.ListMonad.bind /=.
+  rewrite /comp.
+  have: flatten [seq [:: x] | x <- m] = m.
+  { by rewrite (flatten_map1 id) map_id. }
+  by move=> ->.
+Qed.
+
+Definition id_morph : ModelNondet.list ≈≈> ModelNondet.list :=
+  MonadMorphism.Pack _ _ id_nattrans
+    (MonadMorphism.Mixin _ _ id_nattrans ret_id join_id).
+
+Lemma fail_id a : id_morph a Fail = Fail.
+Proof. by []. Qed.
+
+Lemma alt_id a m n : id_morph a (m [~] n) = id_morph a m [~] id_morph a n.
+Proof. by []. Qed.
+
+Definition id_ndmorph : ModelNondet.list ≈> ModelNondet.list :=
+  NDMonadMorphism.Pack _ _ id_morph
+    (NDMonadMorphism.Mixin _ _ id_morph fail_id alt_id).
+
 Lemma path_memF {x p y}: 
-  path (fun x : T => (sfrel f)^~ x) x p ->
+  path (fun x : T => (@sfrel ModelNondet.list id_ndmorph T f)^~ x) x p ->
   y \in p -> y \in F.
 Proof.
-  elim: p x=> //= ?? IHp ? /andP[/memF ? /IHp ?]. 
+  elim: p x=> //= ?? IHp ? /andP[]. rewrite /sfrel /= => /memF ? /IHp ?.
   by rewrite inE=> /orP[/eqP->|].
 Qed.
 
@@ -267,7 +370,7 @@ Proof.
 Qed.
 
 Definition fdfs_path x y : Prop :=
-  exists2 p, path (fun a => sfrel f ^~ a) x p & y = last x p.
+  exists2 p, path (fun a => @sfrel _ id_ndmorph T f ^~ a) x p & y = last x p.
 
 Lemma NmemF x: x \notin F ->
   fdfs n [::] x = [:: x].
@@ -306,7 +409,7 @@ Proof.
       elim/last_ind: p P l=> //= [_ []|????]//.
       by rewrite map_rcons ?last_rcons=> <-.
     apply/(@DfsPath _ _ _ _ _ [seq [`path_memF P (valP z)] | z <- seq_in p]).
-    - rewrite -(rpath equiv _ _ _ (fun x=> (sfrel f)^~ x) p x)/equiv=> //.
+    - rewrite -(rpath equiv _ _ _ (fun x=> (@sfrel _ id_ndmorph T f)^~ x) p x)/equiv=> //.
       - move=>>/eqP->/eqP->; exact/equivs_mem/equivs_hack_f.
       by apply/equivsP; rewrite -map_comp -{1}(val_seq_in p) -eq_in_map.
     - elim/last_ind: p l P=> //= [? _|]; first exact/val_inj.
@@ -328,7 +431,7 @@ Definition t_closure : rel T :=
   fun x y => x \in suffix y.
 
 Lemma rt_closure_n1P x y : 
-  reflect (clos_refl_trans_n1 T (sfrel f) x y) (rt_closure x y).
+  reflect (clos_refl_trans_n1 T (@sfrel _ id_ndmorph T f) x y) (rt_closure x y).
 Proof.
   apply/(equivP (fdfsP y x)); split=> [[p]|].
   - elim: p x y=> //= [>_->|]; first by constructor.
@@ -347,7 +450,7 @@ Arguments clos_t_clos_rt {_ _ _ _}.
 Arguments t1n_trans _ {_ _ _ _}.
 
 Lemma t_closure_n1P x y: 
-  reflect (clos_trans_n1 T (sfrel f) x y) (t_closure x y).
+  reflect (clos_trans_n1 T (@sfrel _ id_ndmorph T f) x y) (t_closure x y).
 Proof.
   apply: (iffP flatten_mapP)=> [[? /rt_closure_n1P /clos_rtn1_rt]|].
   - rewrite clos_refl_transE=> [[? /clos_trans_t1n ? R|]]; last by constructor.
@@ -360,4 +463,3 @@ Qed.
 End FinRTClosure.
 
 End FinClosure.
-
